process/beta.v
@@ -2,15 +2,16 @@ From SST Require Export aux.unscoped aux.expressions process.processes process.s
 Require Import List String Relations ZArith.
 Require Import Setoid Morphisms Coq.Program.Basics.
 Import ListNotations.
+Require Import Coq.Init.Datatypes.
 
 Inductive betaP: relation session :=
   | r_comm  : forall p q xs l e Q M,
-              betaP ((p <-- p_recv q xs) ||| (q <-- p_send p l e Q) ||| M)
-                    ((p <-- subst_expr_proc (p_recv q xs) l e) ||| (q <-- Q) ||| M)
+              betaP ((p <-- Some (p_recv q xs)) ||| (q <-- Some (p_send p l e Q)) ||| M)
+                    ((p <-- subst_expr_proc (p_recv q xs) l e) ||| (q <-- Some Q) ||| M)
   | rt_ite  : forall p P Q M,
-              betaP ((p <-- p_ite (e_val (vbool true)) P Q) ||| M) ((p <-- P) ||| M)
+              betaP ((p <-- Some (p_ite (e_val (vbool true)) P Q)) ||| M) ((p <-- Some P) ||| M)
   | rf_ite  : forall p P Q M,
-              betaP ((p <-- p_ite (e_val (vbool false)) P Q) ||| M) ((p <-- Q) ||| M)
+              betaP ((p <-- Some (p_ite (e_val (vbool false)) P Q)) ||| M) ((p <-- Some Q) ||| M)
   | r_struct: forall M1 M1' M2 M2', scong M1 M1' -> scong M2' M2 -> betaP M1' M2' -> betaP M1 M2.
 
 Declare Instance Equivalence_beta : Equivalence betaP.
@@ -35,9 +36,9 @@ Definition PBob: process :=
 Definition PCarol: process :=
   p_recv "Bob" [(2, sint, p_send "Alice" 3 (e_plus (e_var 0) (e_val (vint 1))) p_inact)].
 
-Definition MS: session := ("Alice" <-- PAlice) ||| ("Bob" <-- PBob) ||| ("Carol" <-- PCarol).
+Definition MS: session := ("Alice" <-- Some PAlice) ||| ("Bob" <-- Some PBob) ||| ("Carol" <-- Some PCarol).
 
-Definition MS': session := ("Alice" <-- p_inact) ||| ("Bob" <-- p_inact) ||| ("Carol" <-- p_inact).
+Definition MS': session := ("Alice" <-- Some p_inact) ||| ("Bob" <-- Some p_inact) ||| ("Carol" <-- Some p_inact).
 
 Eval compute in (eval_expr (e_plus (e_val (vint 100)) (e_val (vint 5)))).
 
@@ -50,8 +51,8 @@ Proof. unfold beta_multistep, MS, MS', PAlice, PBob.
        setoid_rewrite <- sc_par3.
 
        apply multi_step with
-       (y := ((("Bob" <-- p_send "Carol" 2 (e_val (vint 100)) p_inact) |||
-              ("Alice" <-- (p_recv "Carol" [(3, sint, p_inact)]))) ||| ("Carol" <-- PCarol))
+       (y := ((("Bob" <-- Some (p_send "Carol" 2 (e_val (vint 100)) p_inact)) |||
+              ("Alice" <-- Some (p_recv "Carol" [(3, sint, p_inact)]))) ||| ("Carol" <-- Some PCarol))
        ).
        apply r_comm.
        unfold PCarol.
@@ -59,16 +60,16 @@ Proof. unfold beta_multistep, MS, MS', PAlice, PBob.
        setoid_rewrite sc_par2.
        setoid_rewrite <- sc_par3.
        apply multi_step with
-       (y := ((("Carol" <-- p_send "Alice" 3 (e_plus (e_val (vint 100)) (e_val (vint 1)))  p_inact) |||
-              ("Bob" <-- p_inact)) ||| ("Alice" <-- p_recv "Carol" [(3, sint, p_inact)]))
+       (y := ((("Carol" <-- Some (p_send "Alice" 3 (e_plus (e_val (vint 100)) (e_val (vint 1)))  p_inact)) |||
+              ("Bob" <-- Some p_inact)) ||| ("Alice" <-- Some (p_recv "Carol" [(3, sint, p_inact)])))
        ).
        apply r_comm.
 
        setoid_rewrite sc_par2.
        setoid_rewrite <- sc_par3.
        apply multi_step with
-       (y := ((("Alice" <-- p_inact) |||
-              ("Carol" <-- p_inact)) ||| ("Bob" <-- p_inact))
+       (y := ((("Alice" <-- Some p_inact) |||
+              ("Carol" <-- Some p_inact)) ||| ("Bob" <-- Some p_inact))
        ). simpl.
        apply r_comm.
        apply multi_refl.
