process/processes_new.v
@@ -1,0 +1,179 @@
+From SST Require Import aux.unscoped aux.expressions type.global tree.global tree.local.
+Require Import List String Datatypes ZArith Relations.
+Open Scope list_scope.
+From mathcomp Require Import ssreflect.seq.
+Import ListNotations.
+From Paco Require Import paco.
+
+(* Todo: extract P' from muY.P, prove they are the same <- subst and show equal
+      dependecy: fv, fv generator
+      legal types either bottom up constr or top down induct.
+ *)
+
+Section process.
+(* Locally closed approach
+ *)
+Inductive process : Type := 
+  | p_bvar : fin -> process
+  | p_fvar : fin -> process
+  | p_inact : process
+  | p_send : part -> label -> expr -> process -> process
+  | p_recv : part -> list (prod (prod label sort) process) -> process 
+  | p_ite : expr -> process -> process -> process 
+  | p_rec : process -> process.
+  
+
+(* Fixpoint fv (P : process) : list fin := 
+  match P with
+    | p_bvar x => []
+    | p_fvar x => [x]
+    | p_inact => []
+    | p_send p l e P' => fv P'
+    | p_recv p [] => []
+    | p_recv p (((l,s),p') :: xs) => fv (p') ++  fv (p_recv p xs)
+    | p_ite e P1 P2 => fv (P1) ++ fv (P2)
+    | p_rec P' => fv P'
+   end. *)
+(* Compute fv (p_inact).
+Compute (eq_nat 5 6). *)
+
+
+
+(* Definition fresh_free : 
+ *)
+
+(* Helper Function *)
+Fixpoint increase_bound_depth (P: process) : process :=
+  match P with 
+    | p_bvar x => p_bvar (x+1)
+    | p_send p l e P' => p_send p l e (increase_bound_depth P')
+    | p_recv p lis => p_recv p (list_map (fun x => (fst x, increase_bound_depth (snd x))) lis)
+    | p_ite e p1 p2 => p_ite e (increase_bound_depth p1) (increase_bound_depth p2) 
+    | p_rec P' => p_rec (increase_bound_depth P')
+    | _ => P
+  end.
+  
+Fixpoint subst_proc (n : fin) (P : process) (Q: process) : process :=
+  match P with
+    | p_bvar x => p_bvar x 
+    | p_fvar x => if (Nat.eqb x n) then Q else (p_fvar x) 
+    | p_inact => p_inact 
+    | p_send p l e P' => p_send p l e (subst_proc n P' Q)
+    | p_recv p lis => p_recv p (list_map (fun x => (fst x, subst_proc n (snd x) Q)) lis)
+    | p_ite e p1 p2 => p_ite e (subst_proc n p1 Q) (subst_proc n p2 Q)
+    | p_rec P' => p_rec (subst_proc n P' (increase_bound_depth Q))
+  end.
+  
+Compute ((p_rec p_inact) .: p_fvar).
+
+
+Fixpoint subst_proc_bound (P : process) (Q : process) : process := 
+  match P with 
+    | p_bvar x => (Q .: p_bvar) x
+    | p_send p l e P' => p_send p l e (subst_proc_bound P' Q)
+    | p_recv p lis => p_recv p (list_map (fun x => (fst x, subst_proc_bound (snd x) Q)) lis)
+    | p_ite e p1 p2 => p_ite e (subst_proc_bound p1 Q) (subst_proc_bound p2 Q) 
+    | p_rec P' => p_rec (subst_proc_bound P' (increase_bound_depth Q))
+    | _ => P
+  end.
+   
+   
+(*    definition kind of depends on how you want to unfold rec 
+ *)
+ 
+ (* Illegal stuff is allowed, like we can do p_bvar 3 without 4 p_recs on the outside, should probably define locally closed
+   *)
+
+ 
+Fixpoint unfold_rec (P : process) : process :=
+  match P with 
+    | p_send p l e P' => p_send p l e (unfold_rec P')
+    | p_recv p lis => p_recv p (list_map (fun x => (fst x, unfold_rec (snd x))) lis)
+    | p_ite e p1 p2 => p_ite e (unfold_rec p1) (unfold_rec p2)
+    | p_rec P' => subst_proc_bound P' P
+    | _ => P
+  end.
+
+Definition unfold_outer_rec (P : process) : process :=
+  match P with 
+    | p_rec P' => subst_proc_bound P' P
+    | _ => P
+  end.
+
+
+Example simple_mu : process := 
+  p_rec (p_send "Alice" 1 (e_val (vnat 100)) (p_bvar 0)).
+  
+Compute unfold_rec (unfold_rec simple_mu).
+
+Example Pcomplex_mu : process := 
+  p_rec (p_recv "Alice" [
+    (0, sbool, p_bvar 0);
+    (1, sbool, p_rec (p_recv "Bob" [
+       (3, sbool, p_bvar 0);
+       (4, sbool, p_bvar 1);
+       (5, sbool, p_inact)
+    ]));
+    (2, sbool, p_inact)
+  ]).
+  
+
+CoFixpoint Tcomplex_mu : ltt := 
+  ltt_recv "Alice" [
+    (0, sbool, Tcomplex_mu);
+    (1, sbool, complex_mu_1);
+    (2, sbool, ltt_end)
+  ]
+  with complex_mu_1 : ltt :=
+    ltt_recv "Bob" [(3, sbool, Tcomplex_mu); (4, sbool, complex_mu_1); (5, sbool, ltt_end)].
+
+Compute unfold_rec Pcomplex_mu.
+
+
+(* Example _complex_mu_ : typ_proc 0 0 empty Pcomplex_mu Tcomplex_mu.
+Proof. unfold PG_agency.
+  rewrite(ltt_eq TG_agency). simpl.
+  constructor.
+ *)
+
+
+Example recursive_mu : process :=
+  p_rec (p_send "A" 0 (e_val (vnat 1)) (
+    p_rec (p_recv "B" [
+      (1, sbool, p_bvar 0); 
+      (2, sbool, p_send "C" 2 (e_val (vnat 2)) (p_bvar 1))
+    ])
+  )).
+
+Compute unfold_rec recursive_mu.
+
+Example subst_mu : process := 
+  p_rec (p_recv "Alice" [
+    (0, sbool, p_bvar 0);
+    (1, sbool, p_recv "Bob" [
+       (3, sbool, p_bvar 0);
+       (4, sbool, p_fvar 15);
+       (5, sbool, p_fvar 16);
+       (6, sbool, p_inact)
+    ]);
+    (2, sbool, p_inact)
+  ]).
+ 
+Compute subst_proc 15 subst_mu Pcomplex_mu. 
+
+Lemma congr_p_inact  : p_inact  = p_inact  .
+Proof. congruence. Qed.
+
+Lemma congr_p_send  { s0 : part   } { s1 : label   } { s2 : expr   } { s3 : process   } { t0 : part   } { t1 : label   } { t2 : expr   } { t3 : process   } (H1 : s0 = t0) (H2 : s1 = t1) (H3 : s2 = t2) (H4 : s3 = t3) : p_send  s0 s1 s2 s3 = p_send  t0 t1 t2 t3 .
+Proof. congruence. Qed.
+
+Lemma congr_p_recv  { s0 : part   } { s1 : list (prod (prod (label  ) (sort  )) (process  )) } { t0 : part   } { t1 : list (prod (prod (label  ) (sort  )) (process  )) } (H1 : s0 = t0) (H2 : s1 = t1) : p_recv  s0 s1 = p_recv  t0 t1 .
+Proof. congruence. Qed.
+
+Lemma congr_p_ite  { s0 : expr   } { s1 : process   } { s2 : process   } { t0 : expr   } { t1 : process   } { t2 : process   } (H1 : s0 = t0) (H2 : s1 = t1) (H3 : s2 = t2) : p_ite  s0 s1 s2 = p_ite  t0 t1 t2 .
+Proof. congruence. Qed.
+
+Lemma congr_p_rec  { s1 : process   } { t1 : process   }  (H2 : s1 = t1) : p_rec  s1 = p_rec t1 .
+Proof. congruence. Qed.
+
+
