process/sessions.v
@@ -2,10 +2,12 @@ From SST Require Export aux.unscoped aux.expressions process.processes type.glob
 Require Import List String Relations.
 Require Import List String Relations ZArith.
 Require Import Setoid Morphisms Coq.Program.Basics.
+Require Import Coq.Init.Datatypes.
 
 Inductive session: Type :=
-  | s_ind : part   -> process -> session
+  | s_ind : part   -> option process -> session
   | s_par: session -> session -> session.
+  
 
 (* Inductive pcong: relation process :=
   | pc_rec  : forall p, pcong (p_rec p) (subst_process ((p_rec p) .: p_var) p). *)
@@ -14,9 +16,8 @@ Notation "p '<--' P"   :=  (s_ind p P) (at level 50, no associativity).
 Notation "s1 '|||' s2" :=  (s_par s1 s2) (at level 50, no associativity).
 
 Inductive scong: relation session :=
-  | sc_rec  : forall p P M, scong (p <-- (p_rec P) ||| M) (p <-- (subst_process ((p_rec P) .: p_var) P) ||| M)
-(*   | sc_multi: forall p P Q M, pcong P Q -> scong (p <-- P ||| M) (p <-- Q ||| M)  *)
-  | sc_par1 : forall p M, scong (p <-- p_inact ||| M) M
+  | sc_multi: forall p P Q M, scongP P Q -> scong (p <-- Some P ||| M) (p <-- Some Q ||| M) 
+  | sc_par1 : forall p M, scong (p <-- Some p_inact ||| M) M
   | sc_par2 : forall M M', scong (M ||| M') (M' ||| M)
   | sc_par3 : forall M M' M'', scong ((M ||| M') ||| M'') (M ||| (M' ||| M''))
   | sc_par4 : forall M M' M'', scong ((M ||| M') ||| M'') (M ||| (M'' ||| M')).
