process/typecheck_examples.v
@@ -1,0 +1,285 @@
+From SST Require Import aux.unscoped aux.expressions process.processes process.typecheck type.global tree.global tree.local.
+Require Import List String Datatypes ZArith Relations.
+Open Scope list_scope.
+From mathcomp Require Import ssreflect.seq.
+Import ListNotations.
+From Paco Require Import paco.
+
+
+Definition PG_agency : process := p_rec (p_recv "Customer" [(0, sbool, p_send "Customer" 1 (e_val (vnat 5000)) (p_recv "Customer" [
+  (2, sbool, p_recv "Customer" [(3, snat, (p_send "Customer" 4 (e_val (vnat 25122019)) p_inact))]);
+  (5, sbool, p_rec (p_var 0));
+  (6, sbool, p_inact)]));
+        (7, sbool, p_send "Customer" 1 (e_val (vnat 1000)) (p_recv "Customer" [
+  (2, sbool, p_recv "Customer" [(3, snat, (p_send "Customer" 4 (e_val (vnat 25122019)) p_inact))]);
+  (5, sbool, p_rec (p_var 0));
+  (6, sbool, p_inact)]))
+  ]).
+
+CoFixpoint TG_agency : ltt := ltt_recv "Customer" [(0, sbool, ltt_send "Customer" [(1, snat, ltt_recv "Customer" [
+  (2, sbool, ltt_recv "Customer" [(3, snat, ltt_send "Customer" [(4, snat, ltt_end)])]);
+  (5, sbool, TG_agency);
+  (6, sbool, ltt_end)])]);  
+        (7, sbool, ltt_send "Customer" [(1, snat, ltt_recv "Customer" [
+  (2, sbool, ltt_recv "Customer" [(3, snat, ltt_send "Customer" [(4, snat, ltt_end)])]);
+  (5, sbool, TG_agency);
+  (6, sbool, ltt_end)])])].
+
+Example _vgi_agency_ : typ_proc 0 0 empty PG_agency TG_agency.
+Proof. unfold PG_agency.
+  rewrite(ltt_eq TG_agency). simpl.
+  constructor.
+  
+  specialize(tc_recv 1 0 (extendT empty 0
+  (ltt_recv "Customer" [
+    (0, sbool,
+      ltt_send "Customer" [(1, snat,
+      ltt_recv "Customer" [(2, sbool,
+      ltt_recv "Customer" [(3, snat,
+      ltt_send "Customer" [(4, snat, ltt_end)])]);
+      (5, sbool, TG_agency); (6, sbool, ltt_end)])]);
+    (7, sbool,
+      ltt_send "Customer" [(1, snat,
+      ltt_recv "Customer" [(2, sbool,
+      ltt_recv "Customer" [(3, snat,
+      ltt_send "Customer" [(4, snat, ltt_end)])]);
+      (5, sbool, TG_agency); (6, sbool, ltt_end)])])])
+  ) "Customer"
+  [0; 7] 
+  [sbool; sbool]
+  [p_send "Customer" 1 (e_val (vnat 5000)) (
+    p_recv "Customer" [(2, sbool, 
+    p_recv "Customer" [(3, snat, (
+    p_send "Customer" 4 (e_val (vnat 25122019)) p_inact))]);
+    (5, sbool, p_rec (p_var 0));
+    (6, sbool, p_inact)]);
+  p_send "Customer" 1 (e_val (vnat 1000)) (
+    p_recv "Customer" [(2, sbool, 
+    p_recv "Customer" [(3, snat, (
+    p_send "Customer" 4 (e_val (vnat 25122019)) p_inact))]);
+    (5, sbool, p_rec (p_var 0));
+    (6, sbool, p_inact)])
+  ]
+  [ltt_send "Customer" [(1, snat, ltt_recv "Customer" [
+  (2, sbool, ltt_recv "Customer" [(3, snat, ltt_send "Customer" [(4, snat, ltt_end)])]);
+  (5, sbool, TG_agency);
+  (6, sbool, ltt_end)])];
+  ltt_send "Customer" [(1, snat, ltt_recv "Customer" [
+  (2, sbool, ltt_recv "Customer" [(3, snat, ltt_send "Customer" [(4, snat, ltt_end)])]);
+  (5, sbool, TG_agency);
+  (6, sbool, ltt_end)])]]
+  ); intro HR.
+  simpl in HR.
+  apply HR. clear HR. try easy. clear HR. 
+  try easy. clear HR. try easy. clear HR.
+  apply Forall_forall.
+  intros (s, (p, l)) HI0.
+  simpl in HI0.
+  destruct HI0 as [HI0 | HI1].
+  inversion HI0. simpl.
+  subst.
+  constructor.
+  constructor.
+  specialize(tc_recv 1 1 (extendS
+     (extendT empty 0
+        (ltt_recv "Customer"
+           [(0, sbool,
+             ltt_send "Customer"
+               [(1, snat,
+                 ltt_recv "Customer"
+                   [(2, sbool, ltt_recv "Customer" [(3, snat, ltt_send "Customer" [(4, snat, ltt_end)])]);
+                    (5, sbool, TG_agency); (6, sbool, ltt_end)])]);
+            (7, sbool,
+             ltt_send "Customer"
+               [(1, snat,
+                 ltt_recv "Customer"
+                   [(2, sbool, ltt_recv "Customer" [(3, snat, ltt_send "Customer" [(4, snat, ltt_end)])]);
+                    (5, sbool, TG_agency); (6, sbool, ltt_end)])])])) 0 sbool) "Customer"
+      [2; 5; 6]
+      [sbool; sbool; sbool]
+      [
+        p_recv "Customer" [(3, snat, p_send "Customer" 4 (e_val (vnat 25122019)) p_inact)];
+        p_rec (p_var 0);
+        p_inact
+      ]
+      [
+        ltt_recv "Customer" [(3, snat, ltt_send "Customer" [(4, snat, ltt_end)])];
+        TG_agency;
+        ltt_end
+      ]
+   ); intro HR. simpl in HR.
+  apply HR. try easy. try easy. try easy. clear HR. 
+  apply Forall_forall.
+  intros (s, (p, l)) HI1. simpl in HI1.
+  destruct HI1 as [HI1 | HI2].
+  inversion HI1. simpl. subst.
+  specialize(tc_recv 1 2 (extendS
+     (extendS
+        (extendT empty 0
+           (ltt_recv "Customer"
+              [(0, sbool,
+                ltt_send "Customer"
+                  [(1, snat,
+                    ltt_recv "Customer"
+                      [(2, sbool,
+                        ltt_recv "Customer" [(3, snat, ltt_send "Customer" [(4, snat, ltt_end)])]);
+                       (5, sbool, TG_agency); (6, sbool, ltt_end)])]);
+               (7, sbool,
+                ltt_send "Customer"
+                  [(1, snat,
+                    ltt_recv "Customer"
+                      [(2, sbool,
+                        ltt_recv "Customer" [(3, snat, ltt_send "Customer" [(4, snat, ltt_end)])]);
+                       (5, sbool, TG_agency); (6, sbool, ltt_end)])])])) 0 sbool) 1 sbool) "Customer"
+        [3] [snat] [p_send "Customer" 4 (e_val (vnat 25122019)) p_inact] [ltt_send "Customer" [(4, snat, ltt_end)]]
+  ); intro HR. simpl in HR. apply HR.
+  try easy. try easy. try easy. simpl. clear HR. 
+  apply Forall_forall.
+  intros (s, (p, l)) HI2. simpl in HI2.
+  destruct HI2 as [HI2 | HI3].
+  inversion HI2. simpl. subst.
+  constructor.
+  constructor. constructor.
+  simpl.
+  inversion HI3.
+  destruct HI2 as [HI2 | HI3].
+  inversion HI2. subst.
+  constructor. constructor. simpl.
+  rewrite (ltt_eq TG_agency) at 1. simpl. try easy.
+  destruct HI3 as [HI3 | HI4].
+  inversion HI3. subst. 
+  constructor.
+  inversion HI4.
+  destruct HI1 as [HI1 | HI2].
+  inversion HI1. simpl. subst.
+  constructor. constructor. 
+  specialize(tc_recv 1 1 (extendS
+     (extendT empty 0
+        (ltt_recv "Customer"
+           [(0, sbool,
+             ltt_send "Customer"  
+               [(1, snat,
+                 ltt_recv "Customer"
+                   [(2, sbool, ltt_recv "Customer" [(3, snat, ltt_send "Customer" [(4, snat, ltt_end)])]);
+                    (5, sbool, TG_agency); (6, sbool, ltt_end)])]);
+            (7, sbool,
+             ltt_send "Customer"
+               [(1, snat,
+                 ltt_recv "Customer"
+                   [(2, sbool, ltt_recv "Customer" [(3, snat, ltt_send "Customer" [(4, snat, ltt_end)])]);
+                    (5, sbool, TG_agency); (6, sbool, ltt_end)])])])) 0 sbool) "Customer"
+      [2; 5; 6]
+      [sbool; sbool; sbool]
+      [
+        p_recv "Customer" [(3, snat, p_send "Customer" 4 (e_val (vnat 25122019)) p_inact)];
+        p_rec (p_var 0);
+        p_inact
+      ]
+      [
+        ltt_recv "Customer" [(3, snat, ltt_send "Customer" [(4, snat, ltt_end)])];
+        TG_agency;
+        ltt_end
+      ]
+   ); intro HR. simpl in HR.
+  apply HR. try easy. try easy. try easy. clear HR.
+  apply Forall_forall.
+  intros (s, (p, l)) HI4. simpl in HI4.
+  destruct HI4 as [HI4 | HI5].
+  inversion HI4. simpl. subst.
+  specialize(tc_recv 1 2 (extendS
+     (extendS
+        (extendT empty 0
+           (ltt_recv "Customer"
+              [(0, sbool,
+                ltt_send "Customer"
+                  [(1, snat,
+                    ltt_recv "Customer"
+                      [(2, sbool,
+                        ltt_recv "Customer" [(3, snat, ltt_send "Customer" [(4, snat, ltt_end)])]);
+                       (5, sbool, TG_agency); (6, sbool, ltt_end)])]);
+               (7, sbool,
+                ltt_send "Customer"
+                  [(1, snat,
+                    ltt_recv "Customer"
+                      [(2, sbool,
+                        ltt_recv "Customer" [(3, snat, ltt_send "Customer" [(4, snat, ltt_end)])]);
+                       (5, sbool, TG_agency); (6, sbool, ltt_end)])])])) 0 sbool) 1 sbool) "Customer"
+        [3] [snat] [p_send "Customer" 4 (e_val (vnat 25122019)) p_inact] [ltt_send "Customer" [(4, snat, ltt_end)]]
+  ); intro HR. simpl in HR. apply HR.
+  try easy. try easy. try easy. simpl. clear HR. 
+  apply Forall_forall.
+  intros (s, (p, l)) HI5. simpl in HI5.
+  destruct HI5 as [HI5 | HI6].
+  inversion HI5. simpl. subst.
+  constructor.
+  constructor. constructor.
+  simpl.
+  inversion HI6.
+  destruct HI5 as [HI5 | HI6].
+  inversion HI5. simpl. subst. 
+  constructor. constructor. simpl. 
+  rewrite (ltt_eq TG_agency) at 1. simpl. try easy.
+  destruct HI6 as [HI6 | HI7].
+  inversion HI6. subst. simpl. constructor.
+  inversion HI7. inversion HI2.
+
+Qed.
+
+
+Definition PBob2: process := p_rec (p_send "Carol" 2 (e_val (vnat 100)) (p_var 0)).
+CoFixpoint TBob2: ltt := ltt_send "Carol" [(2, snat, TBob2)].
+
+Example newEx: typ_proc 0 0 empty PBob2 TBob2.
+Proof. unfold PBob2.
+       rewrite(ltt_eq TBob2). simpl.
+       constructor.
+       constructor.
+       constructor.
+       constructor.
+       simpl.
+       rewrite(ltt_eq TBob2) at 1. simpl.
+       easy.
+Qed.
+
+
+Definition PTestmu : process := p_rec (p_recv "A" [(0, sbool, p_inact)]).
+Definition TTestmu : ltt := ltt_recv "A" [(0, sbool, ltt_end)].
+
+Example _testmu_1 : typ_proc 0 0 empty PTestmu TTestmu.
+Proof. 
+  unfold PTestmu, TTestmu.
+  specialize(tc_mu 0 0 empty (p_recv "A" [(0, sbool, p_inact)]) (ltt_recv "A" [(0, sbool, ltt_end)])). intro HR.
+  apply HR. clear HR.
+  specialize(tc_recv 1 0 (extendT empty 0 (ltt_recv "A" [(0, sbool, ltt_end)])) "A"
+    [0] [sbool] [p_inact] [ltt_end]
+  ); intro HR.
+  simpl in HR. simpl. apply HR. clear HR. 
+  try easy. clear HR. 
+  try easy. clear HR.
+  try easy. clear HR.
+  apply Forall_forall.
+  intros (s, (p, l)) HIn.
+  simpl in HIn. 
+  destruct HIn as [HIn | HIn].
+  simpl. inversion HIn. 
+  constructor.
+  simpl. inversion HIn.
+Qed.
+
+
+
+  
+Example pr3 : process := p_rec (p_recv "Alice" [
+  (0, sbool, p_var 0);
+  (1, sbool, p_rec (p_recv "Bob" [
+    (2, sbool, p_var 0);
+    (3, sbool, p_var 1);
+    (4, sbool, p_inact)
+    ]))
+  ]).
+  
+
+
+
+
+
